iris/ProofForkretPark.v
@@ -114,6 +114,8 @@ Section Res.
   Definition usertrap_res_bare := FR.usertrap_res_bare.
   Definition usertrap_res_pt_close := FR.usertrap_res_pt_close.
   Definition usertrap_res_pt_open := FR.usertrap_res_pt_open.
+  Definition usertrap_res_ptm_close := FR.usertrap_res_ptm_close.
+  Definition usertrap_res_ptm_open := FR.usertrap_res_ptm_open.
   Definition usertrap_res_bare_norm := FR.usertrap_res_bare_norm.
   Definition usertrap_res_csrs_open := FR.usertrap_res_csrs_open.
   Definition usertrap_res_sstc := FR.usertrap_res_sstc.
